theories/L/TM/TMEncoding.v
@@ -2,7 +2,7 @@ From Undecidability.L.Tactics Require Import LTactics GenEncode.
 From Undecidability.L.Datatypes Require Import LNat Lists LProd LFinType LVector.
 From Undecidability.L Require Import Functions.EqBool.
 
-From Undecidability.TM.Util Require Import VectorPrelim TM_facts.
+From Undecidability.TM.Util Require Import TM_facts.
 
 Require Import Undecidability.Shared.Libs.PSL.FiniteTypes.FinTypes.
 
